[risc-v] support for byte, halfword and word load/store

case_study/RiscvPmpBoundedInts/Base.v
@@ -169,7 +169,14 @@ Inductive CSROP : Set :=
 
 Inductive Retired : Set :=
 | RETIRE_SUCCESS
-| RETIRE_FAIL.
+| RETIRE_FAIL
+.
+
+Inductive WordWidth :=
+| BYTE
+| HALF
+| WORD
+.
 
 Inductive Enums : Set :=
 | privilege
@@ -186,6 +193,7 @@ Inductive Enums : Set :=
 | bop
 | csrop
 | retired
+| wordwidth
 .
 
 Definition RegIdx := bv 3.
@@ -198,8 +206,8 @@ Inductive AST : Set :=
 | BTYPE (imm : bv 13) (rs2 rs1 : RegIdx) (op : BOP)
 | RISCV_JAL (imm : bv 21) (rd : RegIdx)
 | RISCV_JALR (imm : bv 12) (rs1 rd : RegIdx)
-| LOAD (imm : bv 12) (rs1 rd : RegIdx)
-| STORE (imm : bv 12) (rs2 rs1 : RegIdx)
+| LOAD (imm : bv 12) (rs1 rd : RegIdx) (width : WordWidth)
+| STORE (imm : bv 12) (rs2 rs1 : RegIdx) (width : WordWidth)
 | ECALL
 | MRET
 (* Ziscr extension, excluding immediate variants *)
@@ -331,6 +339,7 @@ Section TransparentObligations.
   Derive NoConfusion for BOP.
   Derive NoConfusion for CSROP.
   Derive NoConfusion for Retired.
+  Derive NoConfusion for WordWidth.
   Derive NoConfusion for Unions.
   Derive NoConfusion for AST.
   Derive NoConfusion for ASTConstructor.
@@ -364,6 +373,7 @@ Derive EqDec for UOP.
 Derive EqDec for BOP.
 Derive EqDec for CSROP.
 Derive EqDec for Retired.
+Derive EqDec for WordWidth.
 Derive EqDec for Unions.
 Derive EqDec for AST.
 Derive EqDec for ASTConstructor.
@@ -435,6 +445,10 @@ Section Finite.
     Finite Retired :=
     {| enum := [RETIRE_SUCCESS; RETIRE_FAIL] |}.
 
+  #[export,program] Instance WordWidth_finite :
+    Finite WordWidth :=
+    {| enum := [BYTE; HALF; WORD] |}.
+
   #[export,program] Instance ASTConstructor_finite :
     Finite ASTConstructor :=
     {| enum := [KRTYPE;KITYPE;KUTYPE;KBTYPE;KRISCV_JAL;KRISCV_JALR;KLOAD;KSTORE;KECALL;KMRET;KCSR] |}.
@@ -502,6 +516,7 @@ Module Export RiscvPmpBase <: Base.
   Definition ty_bop                            := (ty.enum bop).
   Definition ty_csrop                          := (ty.enum csrop).
   Definition ty_retired                        := (ty.enum retired).
+  Definition ty_word_width                     := (ty.enum wordwidth).
   Definition ty_mcause                         := (ty_xlenbits).
   Definition ty_exc_code                       := (ty.bvec 8).
   Definition ty_ast                            := (ty.union ast).
@@ -530,6 +545,7 @@ Module Export RiscvPmpBase <: Base.
     | bop              => BOP
     | csrop            => CSROP
     | retired          => Retired
+    | wordwidth        => WordWidth
     end.
 
   Definition union_denote (U : Unions) : Set :=
@@ -576,8 +592,8 @@ Module Export RiscvPmpBase <: Base.
                             | KBTYPE      => ty.tuple [ty.bvec 13; ty_regno; ty_regno; ty_bop]
                             | KRISCV_JAL  => ty.tuple [ty.bvec 21; ty_regno]
                             | KRISCV_JALR => ty.tuple [ty.bvec 12; ty_regno; ty_regno]
-                            | KLOAD       => ty.tuple [ty.bvec 12; ty_regno; ty_regno]
-                            | KSTORE      => ty.tuple [ty.bvec 12; ty_regno; ty_regno]
+                            | KLOAD       => ty.tuple [ty.bvec 12; ty_regno; ty_regno; ty_word_width]
+                            | KSTORE      => ty.tuple [ty.bvec 12; ty_regno; ty_regno; ty_word_width]
                             | KECALL      => ty.unit
                             | KMRET       => ty.unit
                             | KCSR        => ty.tuple [ty_csridx; ty_regno; ty_regno; ty_csrop]
@@ -624,8 +640,8 @@ Module Export RiscvPmpBase <: Base.
                             | BTYPE imm rs2 rs1 op  => existT KBTYPE (tt , imm , rs2 , rs1 , op)
                             | RISCV_JAL imm rd      => existT KRISCV_JAL (tt , imm , rd)
                             | RISCV_JALR imm rs1 rd => existT KRISCV_JALR (tt , imm , rs1 , rd)
-                            | LOAD imm rs1 rd       => existT KLOAD (tt , imm , rs1 , rd)
-                            | STORE imm rs2 rs1     => existT KSTORE (tt , imm , rs2 , rs1)
+                            | LOAD imm rs1 rd w      => existT KLOAD (tt , imm , rs1 , rd , w)
+                            | STORE imm rs2 rs1 w   => existT KSTORE (tt , imm , rs2 , rs1 , w)
                             | ECALL                 => existT KECALL tt
                             | MRET                  => existT KMRET tt
                             | CSR csr rs1 rd op     => existT KCSR (tt , csr , rs1 , rd , op)
@@ -673,8 +689,8 @@ Module Export RiscvPmpBase <: Base.
                               | existT KBTYPE (tt , imm , rs2 , rs1 , op) => BTYPE imm rs2 rs1 op
                               | existT KRISCV_JAL (tt , imm , rd)         => RISCV_JAL imm rd
                               | existT KRISCV_JALR (tt , imm , rs1 , rd)  => RISCV_JALR imm rs1 rd
-                              | existT KLOAD (tt , imm , rs1 , rd)        => LOAD imm rs1 rd
-                              | existT KSTORE (tt , imm , rs2 , rs1)      => STORE imm rs2 rs1
+                              | existT KLOAD (tt , imm , rs1 , rd , w)    => LOAD imm rs1 rd w
+                              | existT KSTORE (tt , imm , rs2 , rs1 , w)  => STORE imm rs2 rs1 w
                               | existT KECALL tt                          => ECALL
                               | existT KMRET tt                           => MRET
                               | existT KCSR (tt , csr , rs1 , rd , op)    => CSR csr rs1 rd op
