theories/Bitvector.v
@@ -602,7 +602,6 @@ Module bv.
 
     Definition msb {n} (v : bv n) : bool :=
       fold_left (fun _ l m => m) false v.
-
   End Access.
 
   Section Extend.
@@ -633,6 +632,11 @@ Module bv.
       match leview m n with is_le k => sext' v k end.
     Definition zext {m} (v : bv m) {n} {p : IsTrue (m <=? n)} : bv n :=
       match leview m n with is_le k => zext' v k end.
+
+    #[program] Definition truncate {n} (m : nat) (xs : bv n) {p : IsTrue (m <=? n)} : bv m :=
+      let (result, _) := appView m (n - m) xs in
+      result.
+    Next Obligation. intros; destruct (leview m n); Lia.lia. Qed.
 
   End Extend.
 
